src/Lean/DenseCheck/Codec.lean
@@ -1,0 +1,61 @@
+import Mathlib.Data.Nat.Pairing
+import DenseCheck.OrderedNodupList
+
+-- open OrderedNodupList
+
+-- Let's open OrderedNodupList
+
+
+universe u
+
+structure Codec  (Rep : Type u) (Value : Type u) where
+  encode : Value → Rep
+  decode : Rep → Value
+  decode_encode : ∀ v, decode (encode v) = v
+  encode_decode : ∀ r, encode (decode r) = r
+
+def Codec.comp
+    {A B C : Type u}
+    (ab : Codec B A)
+    (bc : Codec C B)
+    : Codec C A where
+  encode := fun a => bc.encode (ab.encode a)
+  decode := fun c => ab.decode (bc.decode c)
+  decode_encode := by
+    intro a
+    simp [ab.decode_encode, bc.decode_encode]
+  encode_decode := by
+    intro c
+    simp [ab.encode_decode, bc.encode_decode]
+
+def Codec.xmap
+    {Rep A B : Type u}
+    (c : Codec Rep A)
+    (toB   : A → B)
+    (fromB : B → A)
+    (to_from : ∀ b, toB (fromB b) = b)
+    (from_to : ∀ a, fromB (toB a) = a)
+    : Codec Rep B where
+  encode := fun b => c.encode (fromB b)
+  decode := fun r => toB (c.decode r)
+  decode_encode := by
+    intro b
+    simp [c.decode_encode, to_from]
+  encode_decode := by
+    intro r
+    simp [c.encode_decode, from_to]
+
+
+def NatCodec := Codec Nat
+
+def pairCodec : NatCodec (Nat × Nat) where
+  encode := fun p => Nat.pair p.1 p.2
+  decode := Nat.unpair
+  decode_encode := by simp
+  encode_decode := by simp
+
+def listCodec : Codec Nat (OrderedNodupList Nat) where
+  encode := fun l => l.val.length + 1 + l.val.foldl (fun acc n => acc + n + 1) 0
+  decode := sorry
+  decode_encode := sorry
+  encode_decode := sorry
