src/Lean/DenseCheck/GodelianToolkit.lean
@@ -1,0 +1,78 @@
+import Mathlib.Data.Nat.Pairing
+
+def encodePair (z: Nat) : Nat × Nat :=
+    Nat.unpair z
+
+def decodePair (p: Nat × Nat) : Nat :=
+    let (x, y) := p
+    let m := Nat.max x y
+    m * m + m + x - y
+
+universe u
+
+
+structure NonEmptyList (α : Type u) where
+  head : α
+  tail : List α
+
+def NonEmptyList.toList (α : Type u) (nel : NonEmptyList α) : List α :=
+  nel.head :: nel.tail
+
+def NonEmptyList.length (α : Type u) (nel : NonEmptyList α) : Nat :=
+  1 + nel.tail.length
+
+theorem NonEmptyList.length_pos (α : Type u) (nel : NonEmptyList α) : 0 < nel.length  := by
+  simp [NonEmptyList.length]
+  grind
+
+def NonEmptyList.get {α : Type u} (nel : NonEmptyList α) (n : Fin nel.length) : α :=
+  match n with
+  | ⟨0, _⟩ => nel.head
+  | ⟨Nat.succ k, hk⟩ =>
+      nel.tail.get ⟨k, by sorry⟩
+
+def Endofunction (α : Type u) := α → α
+def NatDecoder (α : Type u) := Nat → α
+def NatEncoder (α : Type u) := α → Nat
+
+def combineChoices
+    (α : Type u)
+    [Inhabited α]
+    (functionList : List ((Nat → α) → Nat → α))
+    (h : functionList.length > 0)
+     : Nat → α :=
+
+  let length := functionList.length
+
+  let rec chooseFunction (fuel : Nat) (n : Nat) (hf : fuel > 0) : α :=
+    -- Can we prove fuel will always be greater than 0?
+    match fuel with
+    | 0 => default
+    | fuel + 1 =>
+        let d := n / length
+        let r := n % length
+        let r : Fin functionList.length := ⟨r, Nat.mod_lt _ (by grind)⟩
+        let f := functionList.get r
+        f (fun m => chooseFunction fuel m (by sorry)) d
+
+  fun n => chooseFunction n.succ n (by grind)
+
+
+inductive Expr
+  | num : Nat → Expr
+  | neg : Expr → Expr
+  | add : Expr → Expr → Expr
+deriving Inhabited
+
+def Nat.toExpression (x : Nat) : Expr :=
+
+  combineChoices (α := Expr)
+    [
+      fun f n => Expr.num n,
+      fun f n => Expr.neg (f n),
+      fun f n => Expr.add (f n) (f n)
+    ]
+    (by decide)
+    x
+
+#eval! Nat.toExpression 345256367
